Definitions for shallow WithPrePost

theories/lang/cpp/specs/spec_notations.v
@@ -3,316 +3,98 @@
  * This software is distributed under the terms of the BedRock Open-Source License.
  * See the LICENSE-BedRock file in the repository root for details.
  *)
-From bedrock.prelude Require Import bytestring telescopes.
-From bedrock.lang.cpp.semantics Require Import values.
-From bedrock.lang.cpp.logic Require Import pred.
-Require Import bedrock.lang.cpp.specs.with_pre_post.
-(* XXX only needed for examples. *)
-Require bedrock.lang.cpp.heap_notations.
-From bedrock.lang.cpp.logic Require heap_pred.
+From bedrock.prelude Require Import bytestring.
 
-Set Universe Polymorphism.
 
-Declare Scope fspec_scope.
-Delimit Scope fspec_scope with fspec.
-Bind Scope fspec_scope with WithPrePost.
+(** Generic Notation *)
+Reserved Notation "'\with' x .. y X"
+   (at level 10, x closed binder, y closed binder, X at level 200, right associativity,
+    format "'[v' '\with'     '[hv' x  ..  y ']'  '//' X ']'").
 
-Section with_Σ.
-  Context `{PROP : bi}.
-
-  #[local] Notation WithPrePost := (WithPrePost PROP) (only parsing).
-
-  Definition add_pre (P : PROP) (wpp : WithPrePost) : WithPrePost :=
-    {| wpp_with := wpp.(wpp_with)
-     ; wpp_pre  := tele_map (fun '(args,X) => (args, P ** X)) wpp.(wpp_pre)
-     ; wpp_post := wpp.(wpp_post)
-     |}.
-
-  Definition add_args (ls : list val) (wpp : WithPrePost) : WithPrePost :=
-    {| wpp_with := wpp.(wpp_with)
-     ; wpp_pre  := tele_map (fun '(args,X) => (ls ++ args, X)) wpp.(wpp_pre)
-     ; wpp_post := wpp.(wpp_post)
-    |}.
-
-  Definition add_arg (s : names.ident) (v : val) (wpp : WithPrePost) : WithPrePost :=
-    {| wpp_with := wpp.(wpp_with)
-     ; wpp_pre  := tele_map (fun '(args,X) => (v :: args, X)) wpp.(wpp_pre)
-     ; wpp_post := wpp.(wpp_post)
-    |}.
-
-  Definition add_post (P : PROP) (wpp : WithPrePost) : WithPrePost :=
-    {| wpp_with := wpp.(wpp_with)
-     ; wpp_pre  := wpp.(wpp_pre)
-     ; wpp_post :=
-         tele_map (WithEx_map (fun r Q => (r,P ** Q))) wpp.(wpp_post)
-    |}.
-
-  Definition add_require (P : Prop) (wpp : WithPrePost) : WithPrePost :=
-    {| wpp_with := wpp.(wpp_with)
-     ; wpp_pre := tele_map (fun '(args,X) => (args, [| P |] ** X)) wpp.(wpp_pre)
-     ; wpp_post := wpp.(wpp_post)
-    |}.
-
-  Definition add_persist (P : PROP) (wpp : WithPrePost) : WithPrePost :=
-    {| wpp_with := wpp.(wpp_with)
-     ; wpp_pre := tele_map (fun '(args,X) => (args, □ P ** X)) wpp.(wpp_pre)
-     ; wpp_post := wpp.(wpp_post)
-    |}.
-
-  Definition add_prepost (P : PROP) (wpp : WithPrePost) : WithPrePost :=
-    add_pre P (add_post P wpp).
-
-  Definition post_void (t : tele) (Q : t -t> PROP) : WithPrePost :=
-    {| wpp_with := TeleO
-     ; wpp_pre := (nil, emp)%I
-     ; wpp_post := {| we_ex := t
-                    ; we_post := tele_map (fun Q => (Vvoid, Q)) Q |} |}.
-
-  Definition post_ret (t : tele) (Q : t -t> val * PROP) : WithPrePost :=
-    {| wpp_with := TeleO
-     ; wpp_pre := (nil, emp)%I
-     ; wpp_post := {| we_ex := t
-                    ; we_post := Q |} |}.
-
-  Definition add_with {t : tele} (wpp : t -t> WithPrePost) : WithPrePost.
-  refine
-    {| wpp_with := tele_append t (tele_map wpp_with wpp)
-     ; wpp_pre  := _
-     ; wpp_post := _
-     |}.
-  { refine ((fix go (t : tele)  :=
-              match t as t
-                    return forall (wpp : t -t> WithPrePost),
-                  tele_append t (tele_map wpp_with wpp) -t> list val * PROP
-              with
-              | TeleO => fun wpp => wpp.(wpp_pre)
-              | TeleS rst => fun wpp x => go (rst x) (wpp x)
-              end) t wpp).
-  }
-  { refine ((fix go (t : tele)  :=
-              match t as t
-                    return forall (wpp : t -t> WithPrePost),
-                  tele_append t (tele_map wpp_with wpp) -t> _
-              with
-              | TeleO => fun wpp => wpp.(wpp_post)
-              | TeleS rst => fun wpp x => go (rst x) (wpp x)
-              end) t wpp).
-  }
-  Defined.
-
-  Definition with_tele (t : telescopes.tele) (f : telescopes.tele_arg t -> WithPrePost)
-  : WithPrePost :=
-    @add_with (telescopes.TeleS (fun x : telescopes.tele_arg t => telescopes.TeleO)) f.
-
-  (* Markers to help notation printing. *)
-  Definition let_fspec (X : WithPrePost) : WithPrePost := X.
-
-  Definition with_arg_fspec (X : WithPrePost) : WithPrePost := X.
-
-  Definition with_pre_fspec (X : WithPrePost) : WithPrePost := X.
-
-  Definition with_prepost_fspec (X : WithPrePost) : WithPrePost := X.
-
-  Definition with_require_fspec (X : WithPrePost) : WithPrePost := X.
-
-  Definition with_persist_fspec (X : WithPrePost) : WithPrePost := X.
-
-  Definition exactWpp (wpp : WithPrePost) : WithPrePost := wpp.
-
-End with_Σ.
-
-Arguments with_tele _ _ _ : clear implicits.
-
-Strategy expand
-   [ add_pre add_args add_require add_arg add_post add_prepost with_tele ].
-(** Make sure to list all identity functions above. And in the same order, for clarity. *)
-Strategy expand
-   [ let_fspec with_arg_fspec with_pre_fspec with_prepost_fspec with_require_fspec with_persist_fspec exactWpp ].
-
-Notation "'\with' x .. y X" :=
-  (@add_with _ (TeleS (fun x => .. (TeleS (fun y => TeleO)) ..))
-            (fun x => .. (fun y => X%fspec) ..))
-  (at level 10, x closed binder, y closed binder, X at level 200, right associativity,
-   format "'[v' '\with'     '[hv' x  ..  y ']'  '//' X ']'").
-
-Notation "'\withT' ts <- t X" := (@with_tele _ t (fun ts => X))
+Reserved Notation "'\withT' ts <- t X"
   (at level 200, ts name, X at level 200, right associativity,
    format "'[v' '\withT'     ts <- t  '//' X ']'").
 
-Notation "'\prepost' pp X" :=
-  (@add_prepost _ pp%I X%fspec)
+Reserved Notation "'\prepost' pp X"
   (at level 10, pp at level 100, X at level 200, right associativity,
    format "'[v' '[hv  ' '\prepost'  '/' pp ']' '//' X ']'").
 
-Notation "'\prepost{' x .. y '}' pp X" :=
-  (with_prepost_fspec ((@add_with _ (TeleS (fun x => .. (TeleS (fun y => TeleO)) .. ))
-                                (fun x => .. (fun y => @add_prepost _ pp%I X%fspec) .. ))))
+Reserved Notation "'\prepost{' x .. y '}' pp X"
   (at level 10, x binder, y binder, pp at level 100, X at level 200, right associativity,
    format "'[v' '[hv  ' '\prepost{' x  ..  y '}'  '/' pp ']' '//' X ']'").
 
-Notation "'\let' x ':=' e X" :=
-  (let_fspec (let x := e in X%fspec))
+Reserved Notation "'\let' x ':=' e X"
   (at level 10, x pattern, e at level 150, X at level 200, right associativity,
    format "'[v' '[hv  ' '\let'      x  ':='  '/' e ']' '//' X ']'").
 
-Notation "'\args' ls X" :=
-  (@add_args _ ls%list X%fspec)
-  (at level 10, X at level 200, right associativity,
-   format "'[v' '[hv  ' '\args'     '/' ls  ']' '//' X ']'").
-
-Notation "'\args{' x .. y '}' ls X" :=
-  (@with_arg_fspec _ (@add_with _ (TeleS (fun x => .. (TeleS (fun y => TeleO)) .. ))
-                                (fun x => .. (fun y => (@add_args _ ls%list X%fspec)) .. )))
-  (at level 10, x binder, y binder, X at level 200, right associativity,
-   format "'[v' '[hv  ' '\args{' x  ..  y '}'  '/' ls  ']' '//' X ']'").
-
-Notation "'\arg' nm v X" :=
-  (@add_arg _ nm%bs v X%fspec)
-  (at level 10, nm at level 0, X at level 200, right associativity,
-   format "'[v' '\arg'  nm  v  '//' X ']'").
-
-Notation "'\arg{' x .. y } nm v X" :=
-  (@with_arg_fspec _ (@add_with _ (TeleS (fun x => .. (TeleS (fun y => TeleO)) ..))
-                                (fun x => .. (fun y => (@add_arg _ nm%bs v X%fspec)) .. )))
-  (at level 10, nm at level 0, x binder, y binder, X at level 200, right associativity,
-   format "'[v' '\arg{' x  ..  y '}'  nm  v  '//' X ']'").
-
-Notation "'\require' pre X" :=
-  (@add_require _ pre X%fspec)
+Reserved Notation "'\require' pre X"
   (at level 10, pre at level 200, X at level 200, left associativity,
    format "'[v' '[' '\require'  pre ']' '//' X ']'").
 
-Notation "'\require{' x .. y } pre X" :=
-  (@with_require_fspec _ (@add_with _ (TeleS (fun x => .. (TeleS (fun y => TeleO)) ..))
-                                (fun x => .. (fun y => (@add_require _ pre X%fspec)) .. )))
+Reserved Notation "'\require{' x .. y } pre X"
   (at level 10, pre at level 200, x binder, y binder, X at level 200, left associativity,
    format "'[v' '\require{' x  ..  y '}'  pre  '//' X ']'").
 
-Notation "'\persist' pre X" :=
-  (@add_persist _ pre%I X%fspec)
+Reserved Notation "'\persist' pre X"
   (at level 10, pre at level 200, X at level 200, left associativity,
    format "'[v' '[' '\persist'  pre ']' '//' X ']'").
 
-Notation "'\persist{' x .. y } pre X" :=
-  (@with_persist_fspec _ (@add_with _ (TeleS (fun x => .. (TeleS (fun y => TeleO)) ..))
-                                (fun x => .. (fun y => (@add_persist _ pre%I X%fspec)) .. )))
+Reserved Notation "'\persist{' x .. y } pre X"
   (at level 10, pre at level 200, x binder, y binder, X at level 200, left associativity,
    format "'[v' '\persist{' x  ..  y '}'  pre  '//' X ']'").
 
-Notation "'\pre' pre X" :=
-  (@add_pre _ pre%I X%fspec)
+Reserved Notation "'\pre' pre X"
   (at level 10, pre at level 200, X at level 200, left associativity,
    format "'[v' '[  ' '\pre'  '/' pre  ']' '//' X ']'").
 
-Notation "'\pre{' x .. y '}' pp X" :=
-  (with_pre_fspec ((@add_with _ (TeleS (fun x => .. (TeleS (fun y => TeleO)) .. ))
-                                (fun x => .. (fun y => @add_pre _ pp%I X%fspec) .. ))))
+Reserved Notation "'\pre{' x .. y '}' pp X"
   (at level 10, x binder, y binder, pp at level 100, X at level 200, right associativity,
    format "'[v' '[hv  ' '\pre{' x  ..  y '}'  '/' pp ']' '//' X ']'").
 
-Notation "'\post' { x .. y } [ r ] post" :=
-  (@post_ret _ (TeleS (fun x => .. (TeleS (fun y => TeleO)) ..))
-             (fun x => .. (fun y => (r, post%I)) ..))
+Reserved Notation "'\post*' post X"
+  (at level 10, post at level 200, X at level 200, left associativity,
+   format "'[v' '[  ' '\post*'  '/' post  ']' '//' X ']'").
+
+Reserved Notation "'\post*{' x .. y '}' post X"
+  (at level 10, x binder, y binder, post at level 100, X at level 200, right associativity,
+   format "'[v' '[hv  ' '\post*{' x  ..  y '}'  '/' post ']' '//' X ']'").
+
+(** Post-conditions with Return *)
+Reserved Notation "'\post' { x .. y } [ r ] post"
   (at level 10, r at level 200, no associativity, x binder, y binder,
    post at level 200,
    format "'[v' '\post' { x  ..  y } [ r ]  '//'          '[hv ' post ']' ']'").
 
-Notation "'\post' { } [ r ] post" :=
-  (@post_ret _ TeleO (r, post%I))
+Reserved Notation "'\post' { } [ r ] post"
   (at level 10, r at level 200, no associativity,
-   post at level 200, only parsing).
+   post at level 200).
 
-Notation "'\post' [ r ] post" :=
-  (@post_ret _ TeleO (r, post%I))
+Reserved Notation "'\post' [ r ] post"
   (at level 10, r at level 200, no associativity,
    post at level 200,
    format "'[v' '\post' [ r ]  '//'          '[hv ' post ']' ']'").
 
-Notation "'\post' post" :=
-  (@post_void _ TeleO post%I)
+Reserved Notation "'\post' post"
   (at level 10, no associativity,
    post at level 200,
    format "'[v' '\post'     '[hv ' post ']' ']'").
 
-Notation "'\exact' wpp" := (exactWpp wpp)
+Reserved Notation "'\exact' wpp"
   (at level 10, wpp at level 200).
 
-Section with_Σ.
-  Context `{Σ : cpp_logic ti}.
+(** Arguments *)
+Reserved Notation "'\args' ls X"
+  (at level 10, X at level 200, right associativity,
+   format "'[v' '[hv  ' '\args'     '/' ls  ']' '//' X ']'").
 
-  Import heap_notations heap_pred.
+Reserved Notation "'\args{' x .. y '}' ls X"
+  (at level 10, x binder, y binder, X at level 200, right associativity,
+   format "'[v' '[hv  ' '\args{' x  ..  y '}'  '/' ls  ']' '//' X ']'").
 
-Goal WithPrePost mpredI.
-refine (
-  \pre emp
-  \post  emp
-).
-(* Show Proof. *)
-Abort.
+Reserved Notation "'\arg' nm v X"
+  (at level 10, nm at level 0, v at level 0, X at level 200, right associativity,
+   format "'[v' '\arg'  nm  v  '//' X ']'").
 
-Goal WithPrePost mpredI.
-refine (
-   \with (I J : mpred) (p : ptr) (R : Qp -> Qp -> nat -> Rep)
-   \prepost emp
-   \require True
-   \require{x} x = 1
-   \arg{n (nn: nat)} "foo" (Vint n)
-   \args{a} [Vint (Z.of_nat a)]
-   \with (z : nat)
-   \prepost emp
-   \prepost{q1 q2} p |-> R q1 q2 0
-   \pre{q3 q4} p |-> R q3 q4 0
-   \pre emp ** Exists y : nat, [| a = 7 |] ** [| y = 3 |] ** I ** J
-   \post {x} [ Vint x ] emp).
-(* Show Proof. *)
-Abort.
-
-Goal WithPrePost mpredI.
-refine (
-   \with (I J : mpred)
-   \with  (a : nat)
-   \prepost emp
-   \with (z : nat)
-   \prepost emp
-   \pre emp ** Exists y : nat, [| a = 7 |] ** [| y = 3 |] ** I ** J
-   \post{r}[ r ] emp).
-(* Show Proof. *)
-Abort.
-
-Goal WithPrePost mpredI.
-refine (
-   \with (I J : mpred) (n : nat)
-   \with  (a : nat)
-   \let x := 3%nat
-   \with (lm : nat * nat)
-   \let (l,m) := lm
-   \require l+m = 3
-   \prepost emp
-   \persist emp
-   \persist{n1} [| n1 = 1 |]
-   \persist{n2} [| n2 = 1 |]%N
-   \persist{z} [| z = 1 |]%Z
-   \with (z : nat)
-   \arg{(zz : Z)} "foo" (Vint zz)
-   \prepost emp
-   \pre emp ** Exists y : nat, [| a = 7 |] ** [| y = 3 |] ** I ** J
-   \post emp).
-(* Show Proof. *)
-Abort.
-
-Goal WithPrePost mpredI.
-refine (
-    \pre emp ** Exists y : nat, [| y = 3 |]
-    \post{}[Vptr nullptr] emp).
-(* Show Proof. *)
-Abort.
-
-
-Goal WithPrePost mpredI.
-refine (
-    \pre |==> True ** |={∅,⊤}=> False
-    \post{}[Vptr nullptr] emp).
-(* Show Proof. *)
-Abort.
-
-End with_Σ.
+Reserved Notation "'\arg{' x .. y } nm v X"
+  (at level 10, nm at level 0, v at level 0, x binder, y binder, X at level 200, right associativity,
+   format "'[v' '\arg{' x  ..  y '}'  nm  v  '//' X ']'").
