theories/lang/cpp/specs/wp_spec_compat.v
@@ -1,0 +1,649 @@
+(*
+ * Copyright (c) 2022 BedRock Systems, Inc.
+ * This software is distributed under the terms of the BedRock Open-Source License.
+ * See the LICENSE-BedRock file in the repository root for details.
+ *)
+Require Import iris.proofmode.tactics.
+Require Import bedrock.lang.algebra.telescopes.
+Require Import bedrock.lang.bi.telescopes.
+Require Import bedrock.lang.cpp.semantics.values.
+Require Import bedrock.lang.cpp.logic.entailsN.
+Require Import bedrock.lang.cpp.specs.classy.
+
+Lemma ex_eq {PROP : bi} {T} (a : T) (P : T -> PROP) :
+  (∃ x : T, [| a = x |] ∗ P x) ⊣⊢ P a.
+Proof.
+  intros. split'.
+  - iIntros "A"; iDestruct "A" as (?) "[-> $]".
+  - iIntros "A"; iExists _; iSplitR; [ | iAssumption ].
+    iPureIntro; eauto.
+Qed.
+
+Lemma ex_eq' {PROP : bi} {T} (a : T) (P : T -> PROP) :
+  (∃ x : T, [| x = a |] ∗ P x) ⊣⊢ P a.
+Proof.
+  intros. split'.
+  - iIntros "A"; iDestruct "A" as (?) "[-> $]".
+  - iIntros "A"; iExists _; iSplitR; [ | iAssumption ].
+    iPureIntro; eauto.
+Qed.
+
+
+Section with_prop.
+  Context {PROP : bi} {ARG : Type} {RESULT : Type}.
+
+  (** The canonical type of function specifications.
+      These are written in weakest pre-condition style which leads to a
+      natural shallow encoding.
+
+      Note that this file goes through some length to maintain backwards
+      compatibility with previous definitions.
+
+      Universes:
+      The universe constraints here are very important note that the universe
+      of the entire type is [bi.u0] which is the universe of the logic. Since
+      the logic is able to quantify over itself, e.g. [forall X : PROP, x], we are
+      free to quantify over specifications without any universe issues. Deeper
+      embeddings of this type do not enjoy this property and can introduce
+      universe subtle universe issues that can be very difficult to debug.
+   *)
+  Record WpSpec : Type@{bi.u0} :=
+    { (* The first three arguments are accumulators that are interpreted away
+         by the [wp_specD] function below.
+         - [acc_arg] is the *reversed* list of arguments that we have seen already
+           We accumulate the list of arguments so that we can assert a *single*
+           equality on all of the arguments.
+         - [acc_pre] is the reversed list of separating conjunctions that have been
+           added to the pre-condition. These are maintained so that they can be
+           placed in the right order and after the equality on the arguments.
+         - [acc_post] is the separating conjunction of propositions that have
+           been added to the post condition.
+         All of these use a deep embedding of a monoid to avoid introducing trivial
+         assertions such as [emp].
+       *)
+      spec_internal : forall (acc_arg : list ARG) (acc_pre : list PROP) (acc_post : list PROP),
+        list ARG -> (RESULT -> PROP) -> PROP
+    ; spec_internal_frame : forall  args' P Q args K K',
+        (∀ r, K r -∗ K' r) ⊢ spec_internal args' P Q args K -∗ spec_internal args' P Q args K'
+      (* the following three fields formally capture the meaning of the accumulators
+       *)
+    ; arg_ok : forall acc_args acc_pre acc_post A args K,
+            spec_internal (acc_args ++ [A]) acc_pre acc_post args K
+        ⊣⊢ (∃ aa, [| args = A :: aa |] ∗ spec_internal acc_args acc_pre acc_post aa K)
+    ; pre_ok : forall acc_args acc_pre acc_post P args K,
+            spec_internal acc_args (P :: acc_pre) acc_post args K
+        ⊣⊢ P ∗ spec_internal acc_args acc_pre acc_post args K
+    ; post_ok : forall acc_args acc_pre acc_post P args K,
+            spec_internal acc_args acc_pre (acc_post ++ [P]) args K
+        ⊣⊢ spec_internal acc_args acc_pre acc_post args (fun x => P -∗ K x)
+    }.
+
+  Lemma spec_internal_proper wp (K K' : _ → PROP) (a : list _) x y z :
+      (forall x, K x ⊣⊢ K' x) ->
+      wp.(spec_internal) x y z a K ⊣⊢ wp.(spec_internal) x y z a K'.
+  Proof.
+    split'.
+    - iIntros "X"; iRevert "X"; iApply spec_internal_frame.
+      iIntros (?). rewrite H. eauto.
+    - iIntros "X"; iRevert "X"; iApply spec_internal_frame.
+      iIntros (?); rewrite H; eauto.
+  Qed.
+
+  Lemma args_ok : forall wp A acc_args acc_pre acc_post args K,
+           wp.(spec_internal) (acc_args ++ A) acc_pre acc_post args K
+      ⊣⊢ (∃ aa, [| args = rev A ++ aa |] ∗ (wp.(spec_internal) acc_args acc_pre acc_post aa K)).
+  Proof.
+    induction A; simpl; intros.
+    - rewrite ex_eq. rewrite app_nil_r. done.
+    - have ->:(acc_args ++ a :: A = (acc_args ++ [a]) ++ A); first by rewrite -assoc.
+      rewrite IHA. setoid_rewrite arg_ok.
+      split'.
+      + iIntros "A"; iDestruct "A" as (aa) "[-> A]"; iDestruct "A" as (aa0) "[-> A]".
+        iExists _; iSplitR; first by iPureIntro; rewrite -assoc; eauto.
+        eauto.
+      + iIntros "A"; iDestruct "A" as (aa) "[-> A]".
+        rewrite -assoc.
+        iExists _; iSplitR; first by iPureIntro; eauto.
+        iExists _; iSplitR; first by iPureIntro; eauto.
+        eauto.
+  Qed.
+
+  Lemma pres_ok : forall wp acc_args acc_pre acc_post P args K,
+          wp.(spec_internal) acc_args (P ++ acc_pre) acc_post args K
+      ⊣⊢ ([∗] P) ∗ wp.(spec_internal) acc_args acc_pre acc_post args K.
+  Proof.
+    intros.
+    induction P; simpl.
+    - by rewrite left_id.
+    - by rewrite pre_ok -assoc IHP.
+  Qed.
+
+  Lemma posts_ok : forall wp P acc_args acc_pre acc_post args K,
+          wp.(spec_internal) acc_args acc_pre (acc_post ++ P) args K
+      ⊣⊢ wp.(spec_internal) acc_args acc_pre acc_post args (fun x => ([∗] P) -∗ K x).
+  Proof.
+    induction P; simpl; intros.
+    - rewrite app_nil_r. apply spec_internal_proper.
+      intros. by rewrite bi.emp_wand.
+    - have ->: (acc_post ++ a :: P = (acc_post ++ [a]) ++ P).
+      { by rewrite -assoc. }
+      rewrite IHP.
+      rewrite post_ok.
+      apply spec_internal_proper.
+      intro.
+      rewrite bi.wand_curry. done.
+  Qed.
+
+  Lemma spec_internal_denote wp acc_arg acc_pre acc_post args K :
+        wp.(spec_internal) acc_arg acc_pre acc_post args K
+    ⊣⊢ ([∗list] P ∈ acc_pre, P) ∗
+           ∃ aa, [| args = rev acc_arg ++ aa |] ∗ wp.(spec_internal) [] [] [] aa (fun x => ([∗list] P ∈ acc_post, P) -∗ K x).
+  Proof.
+    have {1}->: (acc_pre = acc_pre ++ []); first by rewrite app_nil_r.
+    rewrite pres_ok.
+    apply bi.sep_proper; eauto.
+    have {1}->: (acc_post = [] ++ acc_post); first by done.
+    rewrite posts_ok.
+    have {1}->: (acc_arg = [] ++ acc_arg); first by done.
+    by rewrite args_ok.
+  Qed.
+
+  (** The meaning of a [WpSpec] as a weakest pre-condition. *)
+  Definition wp_specD (wpp : WpSpec) : list ARG -> (RESULT -> PROP) -> PROP :=
+    wpp.(spec_internal) nil nil nil.
+
+  Theorem wp_specD_frame (wpp : WpSpec) : forall args Q Q',
+      (∀ r, Q r -∗ Q' r) ⊢ wp_specD wpp args Q -∗ wp_specD wpp args Q'.
+  Proof.
+    intros. apply spec_internal_frame.
+  Qed.
+
+End with_prop.
+#[global,deprecated(since="2022-02-28",note="use [wp_specD_frame]")]
+Notation wpp_frame := (wp_specD_frame) (only parsing).
+
+Arguments WpSpec : clear implicits.
+Coercion wp_specD : WpSpec >-> Funclass.
+
+Module Export wpspec_ofe.
+Section wpspec_ofe.
+  Context {PROP : bi} {ARGS RESULT : Type}.
+  Notation WPP := (WpSpec PROP ARGS RESULT) (only parsing).
+  Instance wpspec_equiv : Equiv WPP :=
+    fun wpp1 wpp2 => forall x Q, wpp1 x Q ≡ wpp2 x Q.
+  Instance wpspec_dist : Dist WPP :=
+    fun n wpp1 wpp2 => forall x Q, wpp1 x Q ≡{n}≡ wpp2 x Q.
+
+  Lemma wpspec_ofe_mixin : OfeMixin WPP.
+  Proof. by apply (iso_ofe_mixin (A := list ARGS -d> (RESULT -> PROP) -d> PROP) wp_specD). Qed.
+  Canonical Structure WpSpecO := Ofe WPP wpspec_ofe_mixin.
+End wpspec_ofe.
+End wpspec_ofe.
+Arguments WpSpecO : clear implicits.
+Notation WithPrePostO PROP := (WpSpecO PROP val val).
+
+(** Universe polYmorphic relations between WPPs. *)
+Definition wpspec_relation {PROP : bi} (R : relation PROP)
+    {ARGS : Type} {RESULT : Type}
+    (wpp1 : WpSpec PROP ARGS RESULT)
+    (wpp2 : WpSpec PROP ARGS RESULT) : Prop :=
+  (** We use a single [K] rather than pointwise equal [K1], [K2] for
+      compatibility with [fs_entails], [fs_impl]. *)
+  forall xs K, R (wpp1 xs K) (wpp2 xs K).
+#[global] Instance: Params (@wpspec_relation) 4 := {}.
+
+Notation wpspec_entailsN n := (wpspec_relation (entailsN n)) (only parsing).
+Notation wpspec_entails := (wpspec_relation bi_entails) (only parsing).
+Notation wpspec_dist n := (wpspec_relation (dist n)) (only parsing).
+Notation wpspec_equiv := (wpspec_relation equiv) (only parsing).
+
+Section wpspec_relations.
+  Context `{!BiEntailsN PROP}.
+
+  Lemma wpspec_equiv_spec {ARGS : Type} {RESULT : Type} wpp1 wpp2 :
+    @wpspec_relation PROP (≡) ARGS RESULT wpp1 wpp2 <->
+    @wpspec_relation PROP (⊢) ARGS RESULT wpp1 wpp2 /\
+    @wpspec_relation PROP (⊢) ARGS RESULT wpp2 wpp1.
+  Proof.
+    split.
+    - intros Hwpp. by split=>vs K; rewrite (Hwpp vs K).
+    - intros [] vs K. by split'.
+  Qed.
+
+  Lemma wpspec_equiv_dist {ARGS : Type} {RESULT : Type} wpp1 wpp2 :
+    @wpspec_relation PROP (≡) ARGS RESULT wpp1 wpp2 <->
+    ∀ n, @wpspec_relation PROP (dist n) ARGS RESULT wpp1 wpp2.
+  Proof.
+    split.
+    - intros Hwpp n vs K. apply equiv_dist, Hwpp.
+    - intros Hwpp vs K. apply equiv_dist=>n. apply Hwpp.
+  Qed.
+
+  Notation entailsN := (@entailsN PROP).
+
+  Lemma wpspec_dist_entailsN {ARGS : Type} {RESULT : Type} wpp1 wpp2 n :
+    @wpspec_relation _ (dist n) ARGS RESULT wpp1 wpp2 <->
+    @wpspec_relation _ (entailsN n) ARGS RESULT wpp1 wpp2 /\
+    @wpspec_relation _ (entailsN n) ARGS RESULT wpp2 wpp1.
+  Proof.
+    split.
+    - intros Hwpp. by split=>vs K; apply dist_entailsN; rewrite (Hwpp vs K).
+    - intros [] vs K. by apply dist_entailsN.
+  Qed.
+
+End wpspec_relations.
+
+Require Import iris.proofmode.tactics.
+
+(** Combinators for building [WpSpec]s *)
+Section with_AR.
+  Context {PROP : bi}.
+  Context {A : Type} {R : Type}.
+
+  #[local] Notation WPP := (WpSpec PROP A R).
+
+  (** [add_with T wpp] adds [T] as logical variable to [wpp] *)
+  #[program] Definition add_with {T : Type@{bi.u2}} (wpp : T -> WPP) : WPP :=
+    {| spec_internal := funI args' P Q args K => ∃ x : T, (wpp x).(spec_internal) args' P Q args K |}.
+  Next Obligation.
+    intros. simpl.
+    iIntros "A B"; iDestruct "B" as (b) "B"; iExists b; iRevert "B"; iApply spec_internal_frame; iAssumption.
+  Qed.
+  Next Obligation.
+    simpl; intros.
+    setoid_rewrite bi.sep_exist_l.
+    rewrite bi.exist_exist.
+    apply bi.exist_proper; intro.
+    rewrite -arg_ok. done.
+  Qed.
+  Next Obligation.
+    simpl; intros.
+    rewrite bi.sep_exist_l.
+    apply bi.exist_proper; intro.
+    by rewrite pre_ok.
+  Qed.
+  Next Obligation.
+    simpl; intros.
+    apply bi.exist_proper; intro.
+    by rewrite post_ok.
+  Qed.
+
+  (** [add_pre P wpp] adds [P] as a pre-condition to [wpp] *)
+  #[program] Definition add_pre (P : PROP) (wpp : WPP) : WPP :=
+    {| spec_internal := funI args' PRE Q args K =>
+         wpp.(spec_internal) args' (P :: PRE) Q args K |}.
+  Next Obligation.
+    intros; simpl; iIntros "A B"; iRevert "B"; iApply spec_internal_frame; iAssumption.
+  Qed.
+  Next Obligation.
+    simpl; intros. by rewrite -arg_ok.
+  Qed.
+  Next Obligation.
+    simpl; intros. do 3 rewrite pre_ok.
+    rewrite assoc (comm _ P) -assoc. done.
+  Qed.
+  Next Obligation.
+    simpl; intros. by rewrite post_ok.
+  Qed.
+
+  (** [add_post P wpp] adds [P] as a post-condition to [wpp]
+
+      TODO: while simple, this produces iterated magic wands rather than a single
+      magic wand, which is much nicer to deal with.
+   *)
+  #[program] Definition add_post (P : PROP) (wpp : WPP) : WPP :=
+    {| spec_internal := funI args' PRE Q  =>
+         wpp.(spec_internal) args' PRE (P :: Q) |}.
+  Next Obligation.
+    simpl; intros.
+    iIntros "A"; by iApply spec_internal_frame.
+  Qed.
+  Next Obligation.
+    simpl; intros. by rewrite arg_ok.
+  Qed.
+  Next Obligation.
+    simpl; intros; by rewrite pre_ok.
+  Qed.
+  Next Obligation.
+    simpl; intros. by rewrite -post_ok.
+  Qed.
+
+  #[global] Instance WpSpec_SpecGen : SpecGen PROP WPP :=
+    {| classy.add_pre := add_pre
+     ; classy.add_post := add_post
+     ; classy.add_with := @add_with |}.
+
+End with_AR.
+
+Section list_arg.
+  Context {PROP : bi}.
+  Context {A : Type}.
+
+  #[local] Notation WPP R := (WpSpec PROP A R).
+
+  Section list_local.
+    Context {T : Type}.
+    #[local] Fixpoint rev_append (ls ls' : list T) : list T :=
+      match ls with
+      | nil => ls'
+      | l :: ls => rev_append ls (l :: ls')
+      end.
+  End list_local.
+
+  (** [add_arg v wpp] adds an argument with value [v] to
+      the beginning of [wpp].
+   *)
+  #[program] Definition add_arg {R} (v : A) (wpp : WPP R) : WPP R :=
+    {| spec_internal := funI args' Q =>
+         wpp.(spec_internal) (v :: args') Q |}.
+  Next Obligation.
+    simpl; intros.
+    iIntros "A"; destruct args'; by iApply spec_internal_frame.
+  Qed.
+  Next Obligation.
+    simpl; intros. by rewrite -arg_ok.
+  Qed.
+  Next Obligation.
+    simpl; intros. by rewrite pre_ok.
+  Qed.
+  Next Obligation.
+    simpl; intros. by rewrite post_ok.
+  Qed.
+
+  #[program] Definition add_args {R} (vs : list A) (wpp : WPP R) : WPP R :=
+    {| spec_internal := funI args' Q =>
+                          wpp.(spec_internal) (rev_append vs args') Q |}.
+  Next Obligation.
+    simpl. intros.
+    iIntros "A"; by iApply spec_internal_frame.
+  Qed.
+  Next Obligation.
+    simpl; intros.
+    change (rev_append vs (acc_args ++ [A0])) with (List.rev_append vs (acc_args ++ [A0])).
+    rewrite rev_append_rev assoc.
+    rewrite arg_ok.
+    rewrite -rev_append_rev. done.
+  Qed.
+  Next Obligation.
+    simpl; intros. by rewrite pre_ok.
+  Qed.
+  Next Obligation.
+    simpl; intros; by rewrite post_ok.
+  Qed.
+
+  #[global] Instance WpSpec_WithArg {R} : WithArg (WPP R) A :=
+    {| classy.add_arg := @add_arg _
+     ; classy.add_args := @add_args _ |}.
+
+End list_arg.
+
+Section post_val.
+  Context {PROP : bi} {ARG : Type} {RESULT : Type}.
+
+  Fixpoint list_sep_into (ls : list PROP) (P : PROP) : PROP :=
+    match ls with
+    | nil => P
+    | l :: ls => list_sep_into ls (l ∗ P) (* l ∗ list_sep_into ls P *)
+    end.
+  Lemma list_sep_into_take : forall ls P,
+      list_sep_into ls P ⊣⊢ P ∗ list_sep_into ls emp.
+  Proof.
+    induction ls; simpl; intros.
+    - split'; eauto. iIntros "[$ _]".
+    - rewrite IHls. symmetry. rewrite IHls. rewrite !assoc bi.sep_emp (comm _ a). done.
+  Qed.
+  #[local] Ltac take_all :=
+    try change @rev_append with List.rev_append ;
+    repeat match goal with
+           | |- context [ list_sep_into _ ?X ] =>
+               lazymatch X with
+               | emp%I => fail
+               | _ => rewrite (list_sep_into_take _ X)
+               end
+           end.
+  Lemma list_sep_into_frame : forall ls P P',
+      (P -∗ P') ⊢ list_sep_into ls P -∗ list_sep_into ls P'.
+  Proof.
+    intros. iIntros "A".
+    take_all.
+    iIntros "[X $]"; iApply "A"; done.
+  Qed.
+  Lemma list_sep_into_app : forall ls ls' P,
+      list_sep_into (ls ++ ls') P ⊣⊢ list_sep_into ls (list_sep_into ls' P).
+  Proof.
+    induction ls; simpl; eauto.
+    intros.
+    rewrite IHls; eauto.
+    take_all.
+    apply bi.sep_proper; eauto.
+    rewrite assoc. apply bi.sep_proper; eauto.
+  Qed.
+  Lemma list_sep_into_rev : forall ls P,
+      list_sep_into (rev ls) P ⊣⊢ list_sep_into ls P.
+  Proof.
+    induction ls; simpl; intros; eauto.
+    rewrite -IHls. rewrite list_sep_into_app.
+    simpl. done.
+  Qed.
+
+  (* We opt to reify this to avoid adding extra equalities when we do not actually need them. arguments that are awkward *)
+  Inductive _post : Type :=
+  | WITH [t : Type@{bi.u2}] (_ : t -> _post)
+  | DONE (_ : RESULT) (_ : PROP).
+
+  Fixpoint _postD (p : _post) (ls : list PROP) (K : RESULT -> PROP) : PROP :=
+    match p with
+    | WITH f => ∀ x, _postD (f x) ls K
+    | DONE r P => list_sep_into ls P -∗ K r
+    end.
+  #[global] Coercion _postD : _post >-> Funclass.
+
+  Lemma _postD_frame p ls : forall K K',
+      (∀ r, K r -∗ K' r) ⊢ _postD p ls K -∗ _postD p ls K'.
+  Proof.
+    induction p; simpl; intros.
+    - iIntros "A B" (?); iApply (H with "A"). eauto.
+    - iIntros "A B C"; iApply "A"; by iApply "B".
+  Qed.
+  Lemma _postD_proper p ls : forall K K',
+      (forall x, K x ⊣⊢ K' x) ->
+      (_postD p ls K ⊣⊢ _postD p ls K').
+  Proof.
+    induction p; simpl; intros.
+    - apply bi.forall_proper; intro; eauto.
+    - apply bi.wand_proper; eauto.
+  Qed.
+
+  #[program] Definition start_post_list (P : _post) : WpSpec PROP ARG RESULT :=
+    {| spec_internal args' PRE POST :=
+      funI args K => [| args = rev_append args' nil |] ∗ list_sep_into PRE (_postD P POST K)
+    |}.
+  Next Obligation.
+    simpl; intros.
+    iIntros "A [$ B]"; iRevert "B"; iApply list_sep_into_frame; iApply _postD_frame; eauto.
+  Qed.
+  Next Obligation.
+    simpl; intros.
+    setoid_rewrite (assoc _ [| _ |] [| _ |]).
+    setoid_rewrite (comm _ [| _ |] [| _ |]).
+    setoid_rewrite <- (assoc _ [| _ |] [| _ |]).
+    rewrite ex_eq'.
+    have ->: (rev_append (acc_args ++ [A]) [] = A :: rev_append acc_args []); eauto.
+    change (@rev_append) with (@List.rev_append).
+    rewrite !rev_append_rev !rev_app_distr /=. done.
+  Qed.
+  Next Obligation.
+    simpl; intros.
+    rewrite assoc (comm _ P0 [| _ |]) -assoc.
+    apply bi.sep_proper; eauto.
+    rewrite list_sep_into_take.
+    symmetry.
+    rewrite list_sep_into_take.
+    rewrite assoc. done.
+  Qed.
+  Next Obligation.
+    simpl; intros.
+    apply bi.sep_proper; eauto.
+    rewrite list_sep_into_take; symmetry; rewrite list_sep_into_take.
+    apply bi.sep_proper; eauto.
+    induction P; simpl.
+    - apply bi.forall_proper; eauto.
+    - rewrite bi.wand_curry. apply bi.wand_proper; eauto.
+      rewrite list_sep_into_app. simpl.
+      rewrite list_sep_into_take; symmetry; rewrite list_sep_into_take.
+      rewrite (comm _ _ P0) assoc. done.
+  Qed.
+
+  #[program,global] Instance WpSpec_WithPost : WithPost PROP (WpSpec PROP ARG RESULT) RESULT :=
+    {| classy.start_post := start_post_list
+     ; post_with := @WITH
+     ; post_ret := @DONE |}.
+
+End post_val.
+
+Section bind.
+  Context {PROP : bi} {ARG ARG' RESULT RESULT' : Type}.
+
+  (** [wp_spec_bind wp a K] effectively forwards to the specification of [wp]
+      evaluated with the arguments [a] and binds the result of the call passing
+      it to [cont].
+
+      This is used to "wrap" a function specification *and produce another type*.
+
+      It is effectively the same as:
+
+      [[
+      \pre{K} wp a K
+      \post{res' ..}[...] K res' ** ...
+      ]]
+
+      where [res'] is the return value of [wp].
+
+      NOTE: This is still experimental.
+   *)
+  #[program] Definition wp_spec_bind (wp : WpSpec PROP ARG RESULT) (a : list ARG)
+             (cont : RESULT -> @_post PROP RESULT')
+    : WpSpec PROP ARG' RESULT' :=
+    {| spec_internal := funI args PRE POST args' K => [| rev_append args nil = args' |] ∗
+                          list_sep_into PRE ((wp a) (fun r => _postD (cont r) POST K))
+    |}.
+  Next Obligation.
+    simpl. intros.
+    iIntros "A [$ B]"; iRevert "B"; iApply list_sep_into_frame.
+    iApply spec_internal_frame.
+    iIntros (?); iApply _postD_frame. done.
+  Qed.
+  Next Obligation.
+    simpl; intros.
+    change @rev_append with List.rev_append.
+    rewrite -!rev_alt.
+    rewrite rev_app_distr/=.
+    split'.
+    - iIntros "[<- A]".
+      iExists _; iSplitR; eauto.
+    - iIntros "A"; iDestruct "A" as (?) "(-> & <- & A)".
+      iSplitR; eauto.
+  Qed.
+  Next Obligation.
+    simpl; intros.
+    rewrite list_sep_into_take; symmetry; rewrite list_sep_into_take.
+    split'.
+    - iIntros "($ & $ & $ & $)".
+    - iIntros "($ & [$ $] & $)".
+  Qed.
+  Next Obligation.
+    simpl; intros.
+    apply bi.sep_proper; eauto.
+    rewrite list_sep_into_take; symmetry; rewrite list_sep_into_take.
+    apply bi.sep_proper; eauto.
+    apply spec_internal_proper. intro.
+    induction (cont x); simpl; eauto.
+    - apply bi.forall_proper; eauto.
+    - rewrite bi.wand_curry. apply bi.wand_proper; eauto.
+      rewrite list_sep_into_app.
+      rewrite list_sep_into_take; symmetry; rewrite list_sep_into_take.
+      simpl.
+      split'.
+      + iIntros "[[$ $] $]".
+      + iIntros "[[$ $] $]".
+  Qed.
+
+  Lemma wp_spec_bind_add_post (P : PROP) spec aargs aas aps aqs args K KONT :
+          spec_internal (wp_spec_bind (add_post P spec) aargs KONT) aas aps aqs args K
+      ⊣⊢ spec_internal (wp_spec_bind spec aargs KONT) aas aps aqs args (funI x => P -∗ K x).
+  Proof.
+    intros. rewrite /wp_spec_bind/=.
+    apply bi.sep_proper; eauto.
+    rewrite list_sep_into_take; symmetry; rewrite list_sep_into_take.
+    apply bi.sep_proper; eauto.
+    change ([P]) with ([] ++ [P]).
+    rewrite post_ok.
+    apply spec_internal_proper.
+    intros.
+    induction KONT; simpl.
+    - split'.
+      + iIntros "A B" (a).
+        iSpecialize ("A" $! a).
+        iRevert "A".
+        iApply _postD_frame.
+        iIntros (?) "A"; iApply "A"; done.
+      + iIntros "A" (a).
+        rewrite H. iIntros "B".
+        iDestruct ("A" with "B") as "A".
+        iApply "A".
+    - split'.
+      + iIntros "A B C". iApply ("A" with "C B").
+      + iIntros "A B C". iApply ("A" with "C B").
+  Qed.
+
+  Lemma wp_spec_bind_add_pre P spec aargs aas aps aqs args K KONT :
+          spec_internal (wp_spec_bind (add_pre P spec) aargs KONT) aas aps aqs args K
+      ⊣⊢ P ∗ spec_internal (wp_spec_bind spec aargs KONT) aas aps aqs args K.
+  Proof.
+    intros. rewrite /wp_spec_bind/=.
+    rewrite list_sep_into_take; symmetry; rewrite list_sep_into_take.
+    rewrite pre_ok.
+    split'.
+    - iIntros "($ & $ & $ & $)".
+    - iIntros "($ & [$ $] & $)".
+  Qed.
+
+  Lemma wp_spec_bind_add_with (T : Type) (spec : T → _) aargs aas aps aqs args K KONT :
+      spec_internal (wp_spec_bind (add_with spec) aargs KONT) aas aps aqs args K
+                    ⊣⊢ (∃ x : T, spec_internal (wp_spec_bind (spec x) aargs KONT) aas aps aqs args K).
+  Proof.
+    intros; simpl.
+    rewrite list_sep_into_take.
+    split'.
+    * iIntros "[$ [A B]]".
+      iDestruct "A" as (a) "A".
+      iExists a. rewrite (list_sep_into_take _ (spec _ _ _)).
+      iFrame.
+    * iIntros "A".
+      iDestruct "A" as (a) "[$ A]".
+      rewrite list_sep_into_take.
+      iDestruct "A" as "[A $]".
+      iExists a. eauto.
+  Qed.
+
+End bind.
+
+
+Lemma spec_add_with {PROP : bi} {ARG RESULT : Type} : forall T (PQ : T -> WpSpec PROP ARG RESULT) args K,
+    (∃ x, wp_specD (PQ x) args K) ⊢ add_with PQ args K.
+Proof.
+  intros; iIntros "A"; iDestruct "A" as (x) "A". iExists x. iApply "A".
+Qed.
+Lemma spec_add_arg {PROP : bi} {ARG RESULT : Type} : forall v (PQ : WpSpec PROP ARG RESULT) args K,
+    match args with
+    | nil => False
+    | v' :: vs => [| v = v' |] ∗ wp_specD PQ vs K
+    end ⊢ add_arg v PQ args K.
+Proof.
+  intros; destruct args; first iIntros "[]".
+  simpl. change ([v]) with (nil ++ [v]).
+  iIntros "[-> A]". rewrite arg_ok. iExists _; iSplitR; eauto.
+Qed.
+
+Arguments list_sep_into {PROP} !_ _/.
+Arguments rev_append {T} !_ _.
